src/Actions/NoOpEnumerator.dfy
@@ -8,10 +8,12 @@ module NoOp {
   import opened Wrappers
   import opened Seq
 
-  class NoOp<T(!new)> extends Action<(), Option<T>> {
+  // Useful test case to ensure it's possible to compose Actions in general:
+  // if you can't simply wrap an Action and implement the same specification,
+  // there's no hope of changing behavior or composing Actions. :)
+  class NoOp<T(!new), R(!new)> extends Action<T, R> {
 
-    const wrapped: Action<(), Option<T>>
-    ghost const wrappedCanProduce: (seq<()>, seq<Option<T>>) -> bool
+    const wrapped: Action<T, R>
       
     ghost predicate Valid() 
       reads this, Repr 
@@ -22,16 +24,13 @@ module NoOp {
     {
       && this in Repr
       && ValidComponent(wrapped)
-      && IsEnumerator(wrapped)
       && CanProduce(consumed, produced)
       && consumed == wrapped.consumed
       && produced == wrapped.produced
-      && wrappedCanProduce == wrapped.CanProduce
     }
 
-    constructor(wrapped: Action<(), Option<T>>) 
+    constructor(wrapped: Action<T, R>) 
       requires wrapped.Valid()
-      requires IsEnumerator(wrapped)
       requires wrapped.consumed == [] && wrapped.produced == []
       ensures Valid()
     { 
@@ -41,28 +40,23 @@ module NoOp {
       produced := [];
       Repr := {this} + wrapped.Repr;
       height := wrapped.height + 1;
-      wrappedCanProduce := wrapped.CanProduce;
       new;
-      assert ValidWrappedProduced(consumed, produced, wrapped.produced);
     }
 
-    ghost predicate CanConsume(consumed: seq<()>, produced: seq<Option<T>>, next: ())
+    ghost predicate CanConsume(consumed: seq<T>, produced: seq<R>, next: T)
+      requires CanProduce(consumed, produced)
       decreases height
     {
-      true
+      wrapped.CanConsume(consumed, produced, next)
     }
-    ghost predicate CanProduce(consumed: seq<()>, produced: seq<Option<T>>)
+
+    ghost predicate CanProduce(consumed: seq<T>, produced: seq<R>)
       decreases height
     {
-      exists producedByWrapped: seq<Option<T>> :: ValidWrappedProduced(consumed, produced, producedByWrapped)
+      wrapped.CanProduce(consumed, produced)
     }
 
-    ghost predicate ValidWrappedProduced(consumed: seq<()>, produced: seq<Option<T>>, producedByWrapped: seq<Option<T>>) {
-      && wrappedCanProduce(consumed, producedByWrapped)
-      && produced == producedByWrapped
-    }
-
-    method Invoke(t: ()) returns (r: Option<T>) 
+    method Invoke(t: T) returns (r: R) 
       requires Valid()
       requires CanConsume(consumed, produced, t)
       modifies Repr
@@ -72,20 +66,31 @@ module NoOp {
       ensures consumed == old(consumed) + [t]
       ensures produced == old(produced) + [r]
     {
-      r := wrapped.Invoke(());
+      r := wrapped.Invoke(t);
 
       Repr := {this} + wrapped.Repr;
       Update(t, r);
-      
-      assert ValidWrappedProduced(consumed, produced, wrapped.produced);
+    }
+  }
+
+  lemma EnumeratornessCommutes<R(!new)>(noop: NoOp<(), Option<R>>)
+    requires noop.Valid()
+    requires IsEnumerator(noop.wrapped)
+    ensures IsEnumerator(noop)
+  {
+    // TODO: working around the fact that triggers don't automatically apply
+    // because noop has the type NoOp as opposed to Action.
+    // Not sure if there's a more reusable workaround to the problem (which is going to recur frequently in this library)
+    var noopAsAction: Action<(), Option<R>> := noop;
+
+    forall consumed, produced, next | noop.CanProduce(consumed, produced) ensures noopAsAction.CanConsume(consumed, produced, next) {
+      assert noop.CanConsume(consumed, produced, next);
     }
 
-    lemma ThisIsEnumerator()
-      requires Valid()
-      ensures IsEnumerator(this)
-    {
-      var limit := EnumerationBound(wrapped);
-      assert EnumerationBoundedBy(this, limit);
+    var limit := EnumerationBound(noop.wrapped);
+    forall consumed: seq<()>, produced: seq<Option<R>> | noopAsAction.CanProduce(consumed, produced) ensures exists n: nat | n <= limit :: Terminated(produced, None, n) {
+      assert noop.CanProduce(consumed, produced);
     }
+    assert EnumerationBoundedBy(noop, limit);
   }
 }
