src/Actions/FunctionAction.dfy
@@ -1,0 +1,81 @@
+
+include "Enumerators.dfy"
+
+module Mapped {
+
+  import opened Actions
+  import opened Enumerators
+  import opened Wrappers
+  import opened Seq
+
+  class FunctionAction<T, R> extends Action<T, R> {
+
+    // TODO: Can we support ~>?
+    const f: T --> R
+
+    ghost predicate Valid()
+      reads this, Repr 
+      ensures Valid() ==> this in Repr 
+      ensures Valid() ==> 
+        && CanProduce(consumed, produced)
+      decreases height, 0
+    {
+      && this in Repr
+      && CanProduce(consumed, produced)
+      && produced == Seq.Map(f, consumed)
+    }
+
+    constructor(f: T -> R) 
+      ensures Valid()
+      ensures this.f == f
+      ensures fresh(Repr)
+      ensures consumed == []
+    { 
+      this.f := f;
+
+      consumed := [];
+      produced := [];
+      Repr := {this};
+    }
+
+    ghost predicate CanConsume(consumed: seq<T>, produced: seq<R>, next: T)
+      requires CanProduce(consumed, produced)
+      decreases height
+    {
+      f.requires(next)
+    }
+    ghost predicate CanProduce(consumed: seq<T>, produced: seq<R>)
+      decreases height
+    {
+      && (forall t <- consumed :: f.requires(t))
+      && produced == Seq.Map(f, consumed)
+    }
+
+    method Invoke(t: T) returns (r: R) 
+      requires Valid()
+      requires CanConsume(consumed, produced, t)
+      modifies Repr
+      decreases height
+      ensures Valid()
+      ensures fresh(Repr - old(Repr))
+      ensures consumed == old(consumed) + [t]
+      ensures produced == old(produced) + [r]
+    {
+      r := f(t);
+
+      Update(t, r);
+    }
+  }
+
+  method Example() {
+    var doubler := new FunctionAction(v => v + v);
+    
+    assert doubler.consumed == [];
+    assert doubler.produced == [];
+    
+    var x := doubler.Invoke(2);
+    assert doubler.produced == [x];
+    assert [x] == [4];
+    assert x == 4;
+  }
+}
